revise implementation of probe operations to use out parameters, generating cleaner C code

src/3d/prelude/EverParse3d.ProbeActions.fst
@@ -9,11 +9,8 @@ module U32 = FStar.UInt32
 module U64 = FStar.UInt64
 open EverParse3d.CopyBuffer
 open LowStar.Buffer
+open LowStar.BufferOps
 open FStar.HyperStack.ST
-
-type maybe a =
-  | Nothing
-  | Just of a
 
 let probe_fn = src:U64.t -> len:U64.t -> dest:copy_buffer_t ->
   Stack bool
@@ -80,13 +77,19 @@ let coerce_value_t (t0 t1:Type0) = t0 -> t1
 
 inline_for_extraction
 let probe_and_read_at_offset_t (t:Type0) (size_t:U64.t) =
+  failed:B.pointer bool ->
   read_offset:U64.t ->
   src:U64.t ->
-  Stack (maybe t)
-    (fun h0 -> True)
-    (fun h0 _ h1 -> 
-      U64.fits (U64.v read_offset + U64.v size_t) /\
-      h0 == h1)
+  Stack t
+    (fun h0 ->
+      B.live h0 failed /\
+      B.get h0 failed 0 == false)
+    (fun h0 _ h1 ->
+      B.live h1 failed /\ 
+      B.modifies (B.loc_buffer failed) h0 h1 /\ (
+        let has_failed = B.get h1 failed 0 in
+        not has_failed ==> U64.fits (U64.v read_offset + U64.v size_t)
+      ))
 
 inline_for_extraction
 let probe_and_read_at_offset_uint32 = probe_and_read_at_offset_t U32.t 4uL
@@ -102,121 +105,136 @@ inline_for_extraction
 let write_at_offset_uint64 = write_at_offset_t U64.t 8uL
 
 
-type probe_m_result a = {
-  next_read_offset:  U64.t;
-  next_write_offset: U64.t;
-  result: maybe a;
-}
 inline_for_extraction
-noextract
-let failed #a (r:probe_m_result a) = 
-  match r.result with
-  | Nothing -> true
-  | _ -> false
+type probe_m_result a = a
 
 inline_for_extraction
 let probe_m a =
-  read_offset:U64.t ->
-  write_offset:U64.t ->
+  read_offset:B.pointer U64.t ->
+  write_offset:B.pointer U64.t ->
+  failed:B.pointer bool ->
   src:U64.t ->
   dest:copy_buffer_t ->
   Stack (probe_m_result a)
     (fun h0 ->
+      B.live h0 read_offset /\
+      B.live h0 write_offset /\
+      B.live h0 failed /\
+      B.disjoint read_offset write_offset /\
+      B.disjoint read_offset failed /\
+      B.disjoint write_offset failed /\
+      B.loc_disjoint
+        (B.loc_union
+          (B.loc_buffer failed) 
+          (B.loc_union
+            (B.loc_buffer read_offset)
+            (B.loc_buffer write_offset)))
+        (loc_of dest) /\
+      B.get h0 failed 0 == false /\
       I.live (stream_of dest) h0)
     (fun h0 res h1 ->
       let sl = stream_of dest in
       I.live sl h1 /\
-      U64.(res.next_write_offset >=^ write_offset) /\
-      U64.(res.next_read_offset >=^ read_offset) /\
-      (if res.next_write_offset <> write_offset
-       then
-        modifies (I.footprint sl) h0 h1 /\
-        (not (failed res) ==> Seq.length (I.get_read sl h1) == 0)
-      else h0 == h1))
+      B.live h1 read_offset /\
+      B.live h1 write_offset /\
+      B.live h1 failed /\
+      (
+        let r0 = B.get h0 read_offset 0 in
+        let r1 = B.get h1 read_offset 0 in
+        let w0 = B.get h0 write_offset 0 in
+        let w1 = B.get h1 write_offset 0 in
+        let has_failed = B.get h1 failed 0 in
+        U64.(w1 >=^ w0) /\
+        U64.(r1 >=^ r0) /\
+        (w0=w1 ==> Seq.length (I.get_read sl h1) == Seq.length (I.get_read sl h0)) /\
+        (w0<>w1 ==> Seq.length (I.get_read sl h1) == 0) /\
+        modifies 
+            (B.loc_union 
+              (B.loc_union 
+                (B.loc_buffer failed)
+                (B.loc_union 
+                  (B.loc_buffer read_offset)
+                  (B.loc_buffer write_offset)))
+              (I.footprint sl)) h0 h1))
 
 inline_for_extraction
 noextract
 let probe_fn_incremental_as_probe_m (f:probe_fn_incremental) (bytes_to_read:U64.t { bytes_to_read <> 0uL}) 
 : probe_m unit
-= fun read_offset write_offset src dest ->
+= fun read_offset write_offset failed src dest ->
     let h0  = get () in
-    let ok = f bytes_to_read read_offset write_offset src dest in
+    let rd = !*read_offset in
+    let wr = !*write_offset in
+    let ok = f bytes_to_read rd wr src dest in
     let h1 = get () in
     if ok
-    then
-      {
-        next_read_offset  = U64.(read_offset +^ bytes_to_read);
-        next_write_offset = U64.(write_offset +^ bytes_to_read);
-        result = Just ()
-      }
-    else
-      {
-        next_read_offset  = read_offset;
-        next_write_offset = write_offset;
-        result = Nothing;
-      }
+    then (
+      read_offset *= U64.(rd +^ bytes_to_read);
+      write_offset *= U64.(wr +^ bytes_to_read)
+    )
+    else (
+      failed *= true
+    )
 
 inline_for_extraction
 noextract
 let write_at_offset_m (#t:Type0) (#w:U64.t { w <> 0uL }) (f:write_at_offset_t t w) (v:t)
 : probe_m unit
-= fun read_offset write_offset src dest ->
-    let ok = f v write_offset dest in
+= fun read_offset write_offset failed src dest ->
+    let wr = !*write_offset in
+    let ok = f v wr dest in
     if ok
     then (
-      {
-        next_read_offset  = read_offset;
-        next_write_offset = U64.(write_offset +^ w);
-        result = Just ()
-      }
+      write_offset *= U64.(wr +^ w)
     )
     else (
-      {
-        next_read_offset  = read_offset;
-        next_write_offset = write_offset;
-        result = Nothing
-      }
+      failed *= true
     )
 
 inline_for_extraction
 noextract
 let probe_and_read_at_offset_m (#t:Type0) (#s:U64.t { s <> 0uL }) (reader:probe_and_read_at_offset_t t s)
 : probe_m t
-= fun read_offset write_offset src dest ->
-  let v = reader read_offset src in
-  match v with
-  | Nothing ->
-    { next_read_offset = read_offset; next_write_offset = write_offset; result = Nothing }
-  | Just v ->
-    { next_read_offset = U64.(read_offset +^ s); next_write_offset = write_offset; result = Just v }
+= fun read_offset write_offset failed src dest ->
+    let rd = !*read_offset in
+    let v = reader failed rd src in
+    let has_failed = !*failed in
+    if has_failed then v
+    else (
+      read_offset *= U64.(rd +^ s);
+      v
+    )
 
 inline_for_extraction
 noextract
-let seq_probe_m (#a:Type) (m1:probe_m unit) (m2:probe_m a)
+let seq_probe_m (#a:Type) (dflt:a) (m1:probe_m unit) (m2:probe_m a)
 : probe_m a
-= fun read_offset write_offset src dest ->
-    let res1 = m1 read_offset write_offset src dest in
-    if failed res1
-    then { res1 with result = Nothing }
-    else m2 res1.next_read_offset res1.next_write_offset src dest
+= fun read_offset write_offset failed src dest ->
+    let res1 = m1 read_offset write_offset failed src dest in
+    let has_failed = !*failed in
+    if has_failed
+    then dflt
+    else m2 read_offset write_offset failed src dest
+    // )
+    // if failed res1
+    // then { res1 with result = Nothing }
+    // else m2 res1.next_read_offset res1.next_write_offset src dest
 
 inline_for_extraction
 noextract
-let bind_probe_m (#a #b:Type) (m1:probe_m a) (m2:a -> probe_m b)
+let bind_probe_m (#a #b:Type) (dflt:b) (m1:probe_m a) (m2:a -> probe_m b)
 : probe_m b
-= fun read_offset write_offset src dest ->
-    let res1 = m1 read_offset write_offset src dest in
-    if failed res1
-    then { res1 with result = Nothing }
-    else let Just v = res1.result in
-         m2 v res1.next_read_offset res1.next_write_offset src dest
+= fun read_offset write_offset failed src dest ->
+    let res1 = m1 read_offset write_offset failed src dest in
+    let has_failed = !*failed in
+    if has_failed then dflt
+    else m2 res1 read_offset write_offset failed src dest
 
 inline_for_extraction
 noextract
 let return_probe_m (#a:Type) (v:a)
 : probe_m a
-= fun read_offset write_offset src dest ->
-    { next_read_offset = read_offset; next_write_offset = write_offset; result = Just v }
+= fun read_offset write_offset failed src dest -> v
 
 let pure_external_action t =
   unit -> Stack t (fun _ -> True) (fun h0 _ h1 -> h0==h1)
@@ -225,9 +243,7 @@ inline_for_extraction
 noextract
 let lift_pure_external_action (#a:Type) (f:pure_external_action a)
 : probe_m a
-= fun read_offset write_offset src dest ->
-    let v = f () in
-    { next_read_offset = read_offset; next_write_offset = write_offset; result = Just v }
+= fun read_offset write_offset failed src dest -> f()
 
 let probe_read_t0_and_write_t1
     (t0 t1:Type0)
@@ -237,7 +253,7 @@ let probe_read_t0_and_write_t1
     (writer:write_at_offset_t t1 size_t1)
     (coerce_t0_t1:coerce_value_t t0 t1)
 : probe_m unit
-= bind_probe_m
+= bind_probe_m ()
     (probe_and_read_at_offset_m reader)
     (fun v -> write_at_offset_m writer (coerce_t0_t1 v)) 
 
@@ -250,29 +266,27 @@ let check_overflow_add (x:U64.t) (y:U64.t)
 inline_for_extraction
 let probe_fn_as_probe_m (bytes_to_read:U64.t { bytes_to_read <> 0uL}) (f:probe_fn)
 : probe_m unit
-= fun read_offset write_offset src dest ->
-    if read_offset <> 0uL
-    || write_offset <> 0uL
-    then { next_read_offset = read_offset;
-           next_write_offset = write_offset;
-           result = Nothing }
+= fun read_offset write_offset failed src dest ->
+    let rd = !*read_offset in
+    let wr = !*write_offset in
+    if rd <> 0uL
+    || wr <> 0uL
+    then (
+      failed *= true
+    )
     else ( 
       let h0 = get () in
       let ok = f src bytes_to_read dest in
       let h1 = get () in
       if ok
-      then
-        {
-          next_read_offset  = bytes_to_read;
-          next_write_offset = bytes_to_read;
-          result = Just ()
-        }
-      else
-        {
-          next_read_offset  = read_offset;
-          next_write_offset = write_offset;
-          result = Nothing
-        }
+      then (
+        read_offset *= bytes_to_read;
+        write_offset *= bytes_to_read;
+        ()
+      )
+      else (
+        failed *= true
+      )
     )
 
 inline_for_extraction
@@ -287,7 +301,18 @@ let run_probe_m (m:probe_m unit) (src:U64.t) (dest:copy_buffer_t)
       I.live sl h1 /\
       modifies (I.footprint sl) h0 h1 /\
       (b <> 0uL ==> Seq.length (I.get_read sl h1) == 0))
-= let res = m 0uL 0uL src dest in
-  if failed res
-  then 0uL
-  else res.next_write_offset
+= EverParse3d.CopyBuffer.properties dest;
+  push_frame();
+    let read_offset = alloca 0uL 1ul in
+    let write_offset = alloca 0uL 1ul in
+    let failed = alloca false 1ul in
+    m read_offset write_offset failed src dest;
+    let wr = !*write_offset in
+    let has_failed = !*failed in
+    let res = 
+      if has_failed
+      then 0uL
+      else !*write_offset
+    in
+  pop_frame();
+  res
