src/3d/prelude/EverParse3d.Interpreter.fst
@@ -583,10 +583,10 @@ let rec probe_action_as_probe_m (p:probe_action)
   | Probe_action_simple bytes_to_read probe_fn ->
     PA.probe_fn_as_probe_m bytes_to_read probe_fn
   | Probe_action_seq m1 m2 ->
-    PA.seq_probe_m (atomic_probe_action_as_probe_m m1) (probe_action_as_probe_m m2)
+    PA.seq_probe_m () (atomic_probe_action_as_probe_m m1) (probe_action_as_probe_m m2)
   | Probe_action_let m1 m2 ->
     let k x : PA.probe_m unit = probe_action_as_probe_m (m2 x) in
-    PA.bind_probe_m (atomic_probe_action_as_probe_m m1) k
+    PA.bind_probe_m () (atomic_probe_action_as_probe_m m1) k
 
 (* The type of atomic actions.
 
